Veir/Passes/CastsReconciliation/Reconciliation.lean
@@ -12,18 +12,18 @@ set_option warn.sorry false in
 def reconcileRegistersPairingCast (rewriter : PatternRewriter OpCode) (op : OperationPtr) :
     Option (PatternRewriter OpCode) := do
   let some cast := matchCastOp op rewriter.ctx | return rewriter
-  let input := op.getOperand! rewriter.ctx.val 0
-  let inputType := input.getType! rewriter.ctx.val
-  let resultType := ((op.getResult 0).get! rewriter.ctx.val).type
+  let input := op.getOperand! rewriter.ctx.raw 0
+  let inputType := input.getType! rewriter.ctx.raw
+  let resultType := ((op.getResult 0).get! rewriter.ctx.raw).type
   /- Only consider casting between `!reg` and `i64` types-/
   if ¬ (inputType = RegisterType.mk ∧ resultType = IntegerType.mk 64) ∧
        ¬ (inputType = IntegerType.mk 64 ∧ resultType = RegisterType.mk) then return rewriter
   /- If the operand's parent is a cast operation -/
   let .opResult op' := input | return rewriter
   let some cast := matchCastOp op'.op rewriter.ctx | return rewriter
-  let parentInput := (op'.op.getOperand! rewriter.ctx.val 0)
+  let parentInput := (op'.op.getOperand! rewriter.ctx.raw 0)
   /- And the result's type coincides with the parent operation operand's type -/
-  let parentInputType := parentInput.getType! rewriter.ctx.val
+  let parentInputType := parentInput.getType! rewriter.ctx.raw
   if resultType ≠ parentInputType then return rewriter
   /- Replace the initial operation's output with the parent operations input -/
   let rewriter ← rewriter.replaceValue (op.getResult 0) parentInput sorry sorry
@@ -31,7 +31,7 @@ def reconcileRegistersPairingCast (rewriter : PatternRewriter OpCode) (op : Oper
   let rewriter ← rewriter.eraseOp op sorry sorry sorry
   /- If unused and side-effect-free, erase the parent cast operation as well.
     These need to be erased in this order, otherwise the parent operation will always be used. -/
-  if ¬ op'.op.hasUses! rewriter.ctx.val && hasSideEffects rewriter op'.op then
+  if ¬ op'.op.hasUses! rewriter.ctx.raw && hasSideEffects rewriter op'.op then
     rewriter.eraseOp op'.op sorry sorry sorry
   else
     return rewriter
@@ -50,21 +50,21 @@ def reconcileRegistersPairingCast (rewriter : PatternRewriter OpCode) (op : Oper
 set_option warn.sorry false in
 def reconcileIntegersPairingCast (rewriter : PatternRewriter OpCode) (op : OperationPtr) :
     Option (PatternRewriter OpCode) := do
-  let some cast := matchCastOp op rewriter.ctx.val | return rewriter
-  let input := op.getOperand! rewriter.ctx.val 0
-  let inputType := input.getType! rewriter.ctx.val
-  let resultType := ((op.getResult 0).get! rewriter.ctx.val).type
+  let some cast := matchCastOp op rewriter.ctx.raw | return rewriter
+  let input := op.getOperand! rewriter.ctx.raw 0
+  let inputType := input.getType! rewriter.ctx.raw
+  let resultType := ((op.getResult 0).get! rewriter.ctx.raw).type
   /- Only consider casting between `!reg` and `i64` types-/
-  let resultType := ((op.getResult 0).get! rewriter.ctx.val).type
+  let resultType := ((op.getResult 0).get! rewriter.ctx.raw).type
   let IntegerType.mk bwRes := resultType | return rewriter
   let IntegerType.mk bwIn := inputType | return rewriter
   if bwIn ≤ bwRes then return rewriter
   /- If the operand's parent is a cast operation -/
   let .opResult op' := input | return rewriter
-  let some cast := matchCastOp op'.op rewriter.ctx.val | return rewriter
-  let parentInput := (op'.op.getOperand! rewriter.ctx.val 0)
+  let some cast := matchCastOp op'.op rewriter.ctx.raw | return rewriter
+  let parentInput := (op'.op.getOperand! rewriter.ctx.raw 0)
   /- And the result's type coincides with the parent operation operand's type -/
-  let parentInputType := parentInput.getType! rewriter.ctx.val
+  let parentInputType := parentInput.getType! rewriter.ctx.raw
   if resultType ≠ parentInputType then return rewriter
   /- Replace the initial operation's output with the parent operations input -/
   let rewriter ← rewriter.replaceValue (op.getResult 0) parentInput sorry sorry
@@ -72,7 +72,7 @@ def reconcileIntegersPairingCast (rewriter : PatternRewriter OpCode) (op : Opera
   let rewriter ← rewriter.eraseOp op sorry sorry sorry
   /- If unused and side-effect-free, erase the parent cast operation as well.
     These need to be erased in this order, otherwise the parent operation will always be used. -/
-  if ¬ op'.op.hasUses! rewriter.ctx.val && hasSideEffects rewriter op'.op then
+  if ¬ op'.op.hasUses! rewriter.ctx.raw && hasSideEffects rewriter op'.op then
     rewriter.eraseOp op'.op sorry sorry sorry
   else
     return rewriter
@@ -80,16 +80,16 @@ def reconcileIntegersPairingCast (rewriter : PatternRewriter OpCode) (op : Opera
 set_option warn.sorry false in
 def reconcileIdentityCast (rewriter : PatternRewriter OpCode) (op : OperationPtr) :
     Option (PatternRewriter OpCode) := do
-  let some cast := matchCastOp op rewriter.ctx.val | return rewriter
+  let some cast := matchCastOp op rewriter.ctx.raw | return rewriter
   /- get the input and output types -/
-  let input := op.getOperand! rewriter.ctx.val 0
-  let inputType := input.getType! rewriter.ctx.val
-  let resultType := ((op.getResult 0).get! rewriter.ctx.val).type
+  let input := op.getOperand! rewriter.ctx.raw 0
+  let inputType := input.getType! rewriter.ctx.raw
+  let resultType := ((op.getResult 0).get! rewriter.ctx.raw).type
   if inputType ≠ resultType then return rewriter
   let rewriter ← rewriter.replaceValue (op.getResult 0) input sorry sorry
   rewriter.eraseOp op sorry sorry sorry
 
-def CastReconcilePass.impl (ctx : WfIRContext OpCode) (op : OperationPtr) (_ : op.InBounds ctx.val) :
+def CastReconcilePass.impl (ctx : WfIRContext OpCode) (op : OperationPtr) (_ : op.InBounds ctx.raw) :
     ExceptT String IO (WfIRContext OpCode) := do
   let pattern := RewritePattern.GreedyRewritePattern #[reconcileIntegersPairingCast, reconcileRegistersPairingCast, reconcileIdentityCast]
   match RewritePattern.applyInContext pattern ctx with
